src/Distributions/Base/Interface.dfy
@@ -1,0 +1,18 @@
+/*******************************************************************************
+*  Copyright by the contributors to the Dafny Project
+*  SPDX-License-Identifier: MIT
+*******************************************************************************/
+
+include "../../ProbabilisticProgramming/RandomNumberGenerator.dfy"
+include "Model.dfy"
+
+import opened RandomNumberGenerator
+
+trait Base {
+  ghost var s: RNG
+
+  method {:extern} Coin() returns (b: bool)
+    modifies this
+    ensures BaseModel.CoinModel(old(s)) == (b, s)
+
+}
