src/Distributions/Base/Model.dfy
@@ -1,0 +1,16 @@
+/*******************************************************************************
+*  Copyright by the contributors to the Dafny Project
+*  SPDX-License-Identifier: MIT
+*******************************************************************************/
+
+include "../../ProbabilisticProgramming/RandomNumberGenerator.dfy"
+include "../../ProbabilisticProgramming/Monad.dfy"
+
+module BaseModel {
+  import opened RandomNumberGenerator
+  import opened Monad
+
+  function CoinModel(s: RNG): (bool, RNG) {
+    Monad.Deconstruct(s)
+  }
+}
