src/Distributions/Bernoulli/Correctness.dfy
@@ -1,0 +1,23 @@
+/*******************************************************************************
+*  Copyright by the contributors to the Dafny Project
+*  SPDX-License-Identifier: MIT
+*******************************************************************************/
+
+include "../../Math/MeasureTheory.dfy"
+include "../../ProbabilisticProgramming/RandomNumberGenerator.dfy"
+include "../../ProbabilisticProgramming/Independence.dfy"
+include "Model.dfy"
+
+import opened MeasureTheory
+import opened Independence
+import opened BernoulliModel
+import opened RandomNumberGenerator
+
+lemma {:axiom} ProbBernoulliIsIndepFn(p: Probability)
+  ensures IsIndepFn(ProbBernoulli(p))
+
+lemma {:axiom} BernoulliCorrectness(p: Probability)
+  ensures
+    var e := iset s | ProbBernoulli(p)(s).0;
+    && e in event_space
+    && mu(e) == p
