src/Distributions/Bernoulli/Implementation.dfy
@@ -1,0 +1,59 @@
+/*******************************************************************************
+*  Copyright by the contributors to the Dafny Project
+*  SPDX-License-Identifier: MIT
+*******************************************************************************/
+
+include "../../Math/MeasureTheory.dfy"
+include "Interface.dfy"
+include "Model.dfy"
+
+import opened MeasureTheory
+import opened BernoulliModel
+
+trait Bernoulli__ extends IBernoulli {
+
+  method Bernoulli(p: real) returns (c: bool)
+    modifies this
+    decreases *
+    requires 0.0 <= p <= 1.0
+    ensures ProbBernoulli(p)(old(s)) == (c, s)
+  {
+    var q: Probability := p as real;
+
+    var b := Coin();
+    if b {
+      if q <= 0.5 {
+        return false;
+      } else {
+        q := 2.0 * (q as real) - 1.0;
+      }
+    } else {
+      if q <= 0.5 {
+        q := 2.0 * (q as real);
+      } else {
+        return true;
+      }
+    }
+
+    while true
+      invariant ProbBernoulli(p)(old(s)) == ProbBernoulli(q)(s)
+      decreases *
+    {
+      b := Coin();
+      if b {
+        if q <= 0.5 {
+          return false;
+        } else {
+          q := 2.0 * (q as real) - 1.0;
+        }
+      } else {
+        if q <= 0.5 {
+          q := 2.0 * (q as real);
+        } else {
+          return true;
+        }
+      }
+    }
+  }
+
+}
