src/Distributions/Bernoulli/Interface.dfy
@@ -1,0 +1,19 @@
+/*******************************************************************************
+*  Copyright by the contributors to the Dafny Project
+*  SPDX-License-Identifier: MIT
+*******************************************************************************/
+
+include "../Base/Interface.dfy"
+include "Model.dfy"
+
+import opened BernoulliModel
+
+trait IBernoulli extends Base {
+
+  method Bernoulli(p: real) returns (c: bool)
+    modifies this
+    decreases *
+    requires 0.0 <= p <= 1.0
+    ensures BernoulliModel.ProbBernoulli(p)(old(s)) == (c, s)
+
+}
