src/Distributions/BernoulliExpNeg/Interface.dfy
@@ -1,0 +1,13 @@
+/*******************************************************************************
+*  Copyright by the contributors to the Dafny Project
+*  SPDX-License-Identifier: MIT
+*******************************************************************************/
+
+trait IBernoulliExpNeg {
+
+  method BernoulliExpNeg(gamma: real) returns (c: bool)
+    modifies this
+    decreases *
+    requires gamma >= 0.0
+
+}
