src/Distributions/DiscreteGaussian/Implementation.dfy
@@ -1,0 +1,31 @@
+/*******************************************************************************
+*  Copyright by the contributors to the Dafny Project
+*  SPDX-License-Identifier: MIT
+*******************************************************************************/
+
+include "Interface.dfy"
+
+trait DiscreteGaussian extends IDiscreteGaussian {
+
+  // Based on Algorithm 3 in https://arxiv.org/pdf/2004.00010.pdf; unverified
+  // Note that we take sigma as a parameter, not sigma^2, to avoid square roots.
+  method DiscreteGaussian(sigma: real) returns (y: int)
+    modifies this
+    requires sigma > 0.0
+    decreases *
+  {
+    var t := sigma.Floor + 1;
+    while true
+      decreases *
+    {
+      y := DiscreteLaplace(1, t);
+      var y_abs := if y < 0 then -y else y;
+      var numerator_term := y_abs as real - sigma * sigma / t as real;
+      var c := BernoulliExpNeg(numerator_term * numerator_term / 2.0 / sigma / sigma);
+      if c {
+        return;
+      }
+    }
+  }
+
+}
