src/Distributions/DiscreteGaussian/Interface.dfy
@@ -1,0 +1,18 @@
+/*******************************************************************************
+*  Copyright by the contributors to the Dafny Project
+*  SPDX-License-Identifier: MIT
+*******************************************************************************/
+
+include "../BernoulliExpNeg/Interface.dfy"
+include "../DiscreteLaplace/Interface.dfy"
+
+trait IDiscreteGaussian extends IDiscreteLaplace, IBernoulliExpNeg {
+
+  // Based on Algorithm 3 in https://arxiv.org/pdf/2004.00010.pdf; unverified
+  // Note that we take sigma as a parameter, not sigma^2, to avoid square roots.
+  method DiscreteGaussian(sigma: real) returns (y: int)
+    modifies this
+    requires sigma > 0.0
+    decreases *
+
+}
