src/Distributions/DiscreteLaplace/Interface.dfy
@@ -1,0 +1,19 @@
+/*******************************************************************************
+*  Copyright by the contributors to the Dafny Project
+*  SPDX-License-Identifier: MIT
+*******************************************************************************/
+
+include "../Bernoulli/Interface.dfy"
+include "../Uniform/Interface.dfy"
+include "../BernoulliExpNeg/Interface.dfy"
+
+trait IDiscreteLaplace extends IBernoulli, IUniform, IBernoulliExpNeg {
+
+  // Based on Algorithm 2 in https://arxiv.org/pdf/2004.00010.pdf; unverified
+  method DiscreteLaplace(s: nat, t: nat) returns (z: int)
+    modifies this
+    requires s >= 1
+    requires t >= 1
+    decreases *
+
+}
