src/Distributions/Geometric/Correctness.dfy
@@ -1,0 +1,32 @@
+/*******************************************************************************
+*  Copyright by the contributors to the Dafny Project
+*  SPDX-License-Identifier: MIT
+*******************************************************************************/
+
+include "../../Math/Helper.dfy"
+include "../../ProbabilisticProgramming/Monad.dfy"
+include "../../ProbabilisticProgramming/Independence.dfy"
+include "../../ProbabilisticProgramming/RandomNumberGenerator.dfy"
+include "../../ProbabilisticProgramming/WhileAndUntil.dfy"
+include "Model.dfy"
+include "Correctness.dfy"
+
+import opened WhileAndUntil
+import opened Independence
+import opened RandomNumberGenerator
+
+lemma {:axiom} ProbWhileGeometricTerminates()
+  ensures
+    var fst := (t: (bool, int)) => t.0;
+    ProbWhileTerminates(ProbGeometricIter, fst)
+
+// Equation (4.19)
+lemma {:axiom} ProbGeometricIsIndepFn()
+  ensures IsIndepFn(ProbGeometric())
+
+// Equation (4.20)
+lemma {:axiom} ProbGeometricCorrectness(n: nat)
+  ensures
+    var e := iset s | ProbGeometric()(s).0 == n;
+    && e in event_space
+    && mu(e) == Helper.RealPower(1.0 / 2.0, n + 1)
