src/Distributions/Geometric/Implementation.dfy
@@ -1,0 +1,53 @@
+/*******************************************************************************
+*  Copyright by the contributors to the Dafny Project
+*  SPDX-License-Identifier: MIT
+*******************************************************************************/
+
+include "../../ProbabilisticProgramming/Monad.dfy"
+include "Interface.dfy"
+
+import opened Monad
+
+trait Geometric extends IGeometric {
+
+  method Geometric() returns (c: nat)
+    modifies this
+    decreases *
+    ensures !old(s)(c)
+    ensures forall i | 0 <= i < c :: old(s)(i)
+    ensures s == IterateTail(old(s), c + 1)
+  {
+    c := 0;
+    var b := Coin();
+    assert old(s)(c) == b;
+    assert s == IterateTail(old(s), c + 1);
+    while b
+      decreases *
+      invariant s == IterateTail(old(s), c + 1)
+      invariant b == IterateTail(old(s), c)(0)
+      invariant b == old(s)(c)
+      invariant forall i | 0 <= i < c :: old(s)(i)
+    {
+      var s' := s;
+      var c' := c;
+      var b' := b;
+      assert forall i | 0 <= i < c' :: old(s)(i);
+      assert s' == IterateTail(old(s), c' + 1);
+      assert b' == IterateTail(old(s), c')(0);
+      b := Coin();
+      assert (b, s) == (Head(s'), Tail(s'));
+      assert b == IterateTail(old(s), c' + 1)(0);
+      assert s == Tail(IterateTail(old(s), c' + 1));
+      TailOfIterateTail(old(s), c' + 1);
+      assert s == IterateTail(old(s), (c' + 1) + 1);
+      c := c + 1;
+      assert c == c' + 1;
+      assert old(s)(c') by {
+        assert b';
+      }
+      assert s == IterateTail(old(s), c + 1);
+      assert b == IterateTail(old(s), c)(0);
+    }
+  }
+
+}
