src/Distributions/Geometric/Interface.dfy
@@ -1,0 +1,18 @@
+/*******************************************************************************
+*  Copyright by the contributors to the Dafny Project
+*  SPDX-License-Identifier: MIT
+*******************************************************************************/
+
+include "../../ProbabilisticProgramming/Monad.dfy"
+include "../Base/Interface.dfy"
+
+trait IGeometric extends Base {
+
+  method Geometric() returns (c: nat)
+    modifies this
+    decreases *
+    ensures !old(s)(c)
+    ensures forall i | 0 <= i < c :: old(s)(i)
+    ensures s == Monad.IterateTail(old(s), c + 1)
+
+}
