src/Distributions/Geometric/Model.dfy
@@ -1,0 +1,27 @@
+/*******************************************************************************
+*  Copyright by the contributors to the Dafny Project
+*  SPDX-License-Identifier: MIT
+*******************************************************************************/
+
+include "../../ProbabilisticProgramming/Monad.dfy"
+include "../../ProbabilisticProgramming/WhileAndUntil.dfy"
+include "Correctness.dfy"
+
+import opened Monad
+import opened WhileAndUntil
+
+// Equation (4.18)
+function ProbGeometric(): Hurd<int> {
+  var fst := (t: (bool, int)) => t.0;
+  var f := (t: (bool, int)) => Return(t.1 - 1);
+  ProbWhileGeometricTerminates();
+  var g := ProbWhile(fst, ProbGeometricIter, (true, 0));
+  Bind(g, f)
+}
+
+  // Equation (4.17)
+function ProbGeometricIter(t: (bool, int)): (f: Hurd<(bool, int)>)
+  ensures forall s :: f(s) == ((Head(s), t.1 + 1), Tail(s))
+{
+  Bind(Deconstruct, (b': bool) => Return((b', t.1 + 1)))
+}
