src/Distributions/Uniform/Implementation.dfy
@@ -1,0 +1,54 @@
+/*******************************************************************************
+*  Copyright by the contributors to the Dafny Project
+*  SPDX-License-Identifier: MIT
+*******************************************************************************/
+
+include "../../Math/MeasureTheory.dfy"
+include "../../ProbabilisticProgramming/Monad.dfy"
+include "Interface.dfy"
+include "Model.dfy"
+
+import opened MeasureTheory
+import opened Monad
+import opened UniformModel
+
+trait UniformFoundational extends IUniform {
+  method Uniform(n: nat) returns (u: nat)
+    modifies this
+    decreases *
+    requires n > 0
+    ensures u < n
+    ensures UniformModel.ProbUniform(n)(old(s)) == (u, s)
+  {
+    assume {:axiom} false;
+    u := Unif(n-1);
+    while u >= n
+      decreases *
+      invariant UniformModel.ProbUniform(n)(old(s)) == UniformModel.ProbUnif(n-1)(old(s))
+      invariant (u, s) == UniformModel.ProbUnif(n-1)(old(s))
+    {
+      u := Unif(n-1);
+    }
+  }
+}
+
+trait Unif extends IUnif {
+  method Unif(n: nat) returns (u: nat)
+    modifies this
+    ensures UniformModel.UnifModel(n)(old(s)) == (u, s)
+  {
+    var k := 1;
+    u := 0;
+
+    while k <= n
+      decreases 2*n - k
+      invariant k >= 1
+      invariant UnifAlternativeModel(n)(old(s)) == UnifAlternativeModel(n, k, u)(s)
+    {
+      var b := Coin();
+      k := 2*k;
+      u := if b then 2*u + 1 else 2*u;
+    }
+  }
+
+}
