src/Distributions/Uniform/ImplementationExtern.dfy
@@ -1,0 +1,17 @@
+/*******************************************************************************
+*  Copyright by the contributors to the Dafny Project
+*  SPDX-License-Identifier: MIT
+*******************************************************************************/
+
+include "Interface.dfy"
+
+trait UniformExtern extends IUniform {
+
+  method {:extern} Uniform(n: nat) returns (u: nat)
+    modifies this
+    decreases *
+    requires n > 0
+    ensures u < n
+    ensures UniformModel.ProbUniform(n)(old(s)) == (u, s)
+
+}
