src/Distributions/Uniform/Interface.dfy
@@ -1,0 +1,26 @@
+/*******************************************************************************
+*  Copyright by the contributors to the Dafny Project
+*  SPDX-License-Identifier: MIT
+*******************************************************************************/
+
+include "../Base/Interface.dfy"
+include "Model.dfy"
+
+trait IUniform extends Base, IUnif {
+
+  method Uniform(n: nat) returns (u: nat)
+    modifies this
+    decreases *
+    requires n > 0
+    ensures u < n
+    ensures UniformModel.ProbUniform(n)(old(s)) == (u, s)
+
+}
+
+trait IUnif extends Base {
+
+  method Unif(n: nat) returns (u: nat)
+    modifies this
+    ensures UniformModel.ProbUnif(n)(old(s)) == (u, s)
+
+}
